LeanSorting/Proof.lean
@@ -1,0 +1,122 @@
+import «LeanSorting».Basic
+
+structure Slice (α : Type) where
+  arr : Array α
+  start : ℕ
+  endExclusive : ℕ
+  start_lt_arr_size : start < arr.size
+  endExclusive_le_arr_size : endExclusive ≤ arr.size
+  start_le_endExclusive : start ≤ endExclusive
+
+def Slice.indices [Ord α] (s : Slice α) : Set ℕ :=
+  { i | i ≥ s.start ∧ i < s.endExclusive }
+
+def Slice.non_decreasing [Ord α] (s : Slice α) : Prop :=
+  (i j : ℕ) →
+    (hp : i ∈ s.indices ∧ j ∈ s.indices ∧ i.succ = j) →
+      have : i < s.arr.size := by
+        apply And.left at hp
+        simp [Slice.indices] at hp
+        apply And.right at hp
+        exact (Nat.lt_of_lt_le hp s.endExclusive_le_arr_size)
+      have : j < s.arr.size := by
+        apply And.right at hp
+        apply And.left at hp
+        simp [Slice.indices] at hp
+        apply And.right at hp
+        exact (Nat.lt_of_lt_le hp s.endExclusive_le_arr_size)
+      Ord.compare s.arr[i] s.arr[j] != Ordering.gt
+
+def mergeAdjacentChunksIntoAuxSlice
+    [Ord α]
+    (m₁ : M₁ α)
+    : Slice α :=
+  let m₁' := mergeAdjacentChunksIntoAux m₁
+  have start_lt_arr_size : m₁'.start₁ < m₁'.aux.size := by sorry
+  have endExclusive_le_arr_size : m₁'.end₂ ≤ m₁'.aux.size := by sorry
+  have start_le_endExclusive : m₁'.start₁ ≤ m₁'.end₂ := by sorry
+  {
+    arr := m₁'.aux,
+    start := m₁'.start₁,
+    endExclusive := m₁'.end₂,
+    start_lt_arr_size,
+    endExclusive_le_arr_size,
+    start_le_endExclusive,
+  }
+
+def mergeAdjacentChunksIntoAux_non_decreasing
+    [Ord α]
+    (m₁ : M₁ α)
+    : Prop :=
+  (mergeAdjacentChunksIntoAuxSlice m₁).non_decreasing
+
+def Array.non_decreasing [Ord α] {as : Array α} : Prop :=
+  ∀ i j : Fin as.size,
+    i.val.succ = j.val →
+      Ord.compare as[i] as[j] != Ordering.gt
+
+def Array.permutation_of (as : Array α) (bs : Array α) : Prop :=
+  Multiset.ofList as.data = Multiset.ofList bs.data
+
+def Array.sorting_algorithm [Ord α] (f : Array α → Array α) : Prop :=
+  ∀ arr : Array α,
+      (f arr).non_decreasing
+    ∧ (f arr).permutation_of arr
+
+-- theorem mergeChunksIntoAuxRuns
+--   [Ord α]
+
+
+theorem mergesort_non_decreasing
+    [Inhabited α]
+    [Ord α]
+    {arr : Array α}
+    : arr.mergeSort.non_decreasing := by
+
+  simp [Array.non_decreasing]
+  intro i j
+  intro i_succ_eq_j
+  simp [Array.mergeSort]
+  sorry
+
+theorem mergesort_preserves_elements
+    [Inhabited α]
+    [Ord α]
+    {arr : Array α}
+    : (Array.mergeSort arr).permutation_of arr := by
+  sorry
+
+theorem sorting_algorithm_mergeSort
+    [Inhabited α]
+    [Ord α]
+    : Array.sorting_algorithm Array.mergeSort (α := α) := by
+  simp [Array.sorting_algorithm]
+  intro arr
+  apply And.intro
+  . case left =>
+    exact mergesort_non_decreasing
+  . case right =>
+    exact mergesort_preserves_elements
+
+-- Sketch of proof:
+--
+-- 1. We need to prove that the returned array is in non-decreasing order.
+--
+-- mergeSort runs with chunk size 1, 2, 4, 8, 16, ..., until the chunk
+-- size is ≥ arr.size.
+--
+-- We need to show that when (chunkSize * 2 ≥ arr.size),
+-- it is the case that after running mergeChunksIntoAux, elements
+-- 0..arr.size of aux form a non-decreasing run.
+--
+-- Our induction hypothesis is that for a given chunkSize C (with C < arr.size),
+-- it is the case that after running mergeChunksIntoAux, elements
+-- 0..2C, 2C..4C, 4C..6C, ... and so on each form non-decreasing runs of aux.
+--
+-- When C=1 (our base case), mergeChunksIntoAux checks if the two elements are in order
+-- and swaps them if they are not, so it follows that elements 0..2,
+--
+-- For C>1, we can assume that 0..2C, 2C..4C, 4C..6C, ... and so on form non-decreasing
+-- runs. We then can show that mergeAdjacentChunksIntoAux, when given a non-decreasing run,
+-- merges 0..C and C..2C, 2C..3C and 3C..4C and so on into non-decreasing runs spanning
+-- both.
